\begin{slide}[Covariance]
$$Cov(X,Y) = E((X-EX)(Y-EY) ) = E(XY) - E(X)E(Y)$$
\begin{minipage}{0.5\textwidth}
\begin{align*}
  Cov(X,X) &= Var(X)\\
  Cov(X,Y) &=Cov(Y,X)\\
  Cov(X,c) &=0\\
  Cov(cX,Y)&=c\,Cov(X,Y)\\
  Cov(X,Y+Z)&=Cov(X,Y)+Cov(X,Z)\\
  Var(X +Y) &= Var(X)+Var(Y)+2Cov(X,Y)
\end{align*}
\end{minipage}
\begin{minipage}{0.5\textwidth}
%\footnotetext
\begin{align*}\textstyle 
Cov&\left(\textstyle \sum_{i}a_iX_i,\sum_{i}b_iY_i\right)\\&=\textstyle \sum_{i,j}a_ib_jCov(X_i,X_j)
\\
Var&\left(\textstyle \sum_{i}X_i\right)\\&=\textstyle \sum_{i}Var(X_i)+2\sum_{i,j}Cov(X_i,X_j)
\end{align*}
\end{minipage}
\vspace{20pt}
$$Corr(X,Y) = {Cov(X,Y) \over SD(X)SD(Y)} = Cov\left({X-E\,X \over SD(X) },{Y-E\,Y \over SD(Y) } \right)$$
$$-1\leq Corr(X,Y)\leq 1$$
\end{slide}